src/henkin.lean
@@ -1,0 +1,1099 @@
+/-
+Copyright (c) 2019 The Flypitch Project. All rights reserved.
+Released under Apache 2.0 license as described in the file LICENSE.
+
+Authors: Jesse Han, Floris van Doorn
+-/
+import .completion .language_extension .colimit
+
+-- local attribute [instance, priority 0] classical.prop_decidable
+
+open fol
+
+universes u v
+local infix ` →ᴸ `:10 := Lhom -- \^L
+
+/- Temporarily putting this here because I can't get Lean to recognize Lhom in colimit.lean -/
+namespace colimit
+
+export directed_type
+/- Below we define colimits of languages. These are just fieldwise (and then indexwise)
+   colimits of types, so the proofs are very similar. -/
+
+local infix ` ∘ `:60 := Lhom.comp
+
+structure directed_diagram_language (D : (directed_type.{u})) : Type (max (u+1) (v+1)) :=
+  (obj : D.carrier → (Language.{v}))
+  (mor : ∀{x}, ∀{y}, D.rel x y → (obj x →ᴸ obj y))
+  (h_mor : ∀{x} {y} {z} {f1 : D.rel x y} {f2 : D.rel y z} {f3 : D.rel x z},
+            (mor f3) = (mor f2) ∘ (mor f1)) -- functoriality
+
+export directed_diagram_language
+
+/- Given a directed diagram of languages, we obtain two ℕ-indexed families of
+   directed diagrams of types: one by restricting to functions and one by
+   restricting to relations. -/
+@[reducible]def diagram_functions {D : (directed_type)} {F : (directed_diagram_language D)} (n : ℕ) :
+                      ((directed_diagram D)) :=
+begin
+  refine ⟨by {intro x, exact (obj F x).functions n},_,_⟩,
+  {intros x y edge, have := (F.mor edge).on_function, exact this },
+  {intros, simp only [], have := F.h_mor, have := @this x y z f1 f2 f3, rw[this]},
+end
+
+@[reducible]def diagram_relations {D : (directed_type)} {F : (directed_diagram_language D)} (n : ℕ) :
+                      ((directed_diagram D)) :=
+begin
+  refine ⟨by {intro x, exact (obj F x).relations n},_,_⟩,
+  {intros x y edge, have := (F.mor edge).on_relation, exact @this n},
+  {intros, simp only [], have := F.h_mor, have := @this x y z f1 f2 f3, rw[this]},
+end
+
+def coproduct_of_directed_diagram_language {D : (directed_type : Type (u+1)) }
+    (F : (directed_diagram_language D :  Type (max (u+1) (v+1)))) :  Language :=
+⟨λn, coproduct_of_directed_diagram (@diagram_functions D F n),
+  λn, coproduct_of_directed_diagram (@diagram_relations D F n)⟩
+
+def colimit_language {D : (directed_type : Type (u+1)) } (F : (directed_diagram_language D)) : Language :=
+⟨λn, @quotient (coproduct_of_directed_diagram (@diagram_functions D F n))
+  ⟨germ_relation (diagram_functions n), germ_equivalence (diagram_functions n)⟩,
+λn, @quotient (coproduct_of_directed_diagram (@diagram_relations D F n))
+  ⟨germ_relation (diagram_relations n), germ_equivalence (diagram_relations n)⟩⟩
+
+/- The canonical map of languages is the pointwise canonical map of colimits of types -/
+def canonical_map_language {D} {F : directed_diagram_language D} (i : D.carrier) :
+                           (F.obj i) →ᴸ colimit_language F :=
+⟨λ n, function.comp (by apply quotient.mk) (@canonical_inclusion_coproduct D (diagram_functions n) i),
+λ n, function.comp (by apply quotient.mk) (@canonical_inclusion_coproduct D (diagram_relations n) i)⟩
+
+-- structure cocone_language' {D} (F : directed_diagram_language D) :=
+--   (vertex : Language)
+--   (cocone_functions : ∀{n}, @colimit.cocone D (@diagram_functions D F n)
+-- would need extra hypotheses that for every n, the vertex of the cocone_functions (resp. relations)
+-- is equal to vertex.functions (resp. relations)
+-- maybe that would have been easier to work with
+
+structure cocone_language {D} (F : directed_diagram_language D) :=
+  (vertex : Language)
+  (map : Π i : D.carrier, F.obj i →ᴸ vertex)
+  (h_compat : ∀{i}, ∀{j}, Π h : D.rel i j, (map i ) = (map j) ∘ (F.mor h))
+
+export cocone_language
+
+def cocone_of_colimit_language {D} (F : directed_diagram_language D) : cocone_language F :=
+begin
+  refine ⟨colimit_language F, canonical_map_language, _⟩, intros i j H, fapply Lhom.Lhom_funext,
+  all_goals{fapply funext, intro n,
+  simp only [quotient.eq,(≈),canonical_map_language,function.comp], have h_refl : D.rel j j,
+  by apply D.h_reflexive, -- refine ⟨j,F.mor H x, H, h_refl, rfl, _⟩,
+  fapply funext, intro x, simp only [quotient.eq,(≈),canonical_map_language,function.comp],
+  },
+  {refine ⟨j,(F.mor H).on_function x, H, h_refl, rfl, _⟩,
+  change (function.comp ((diagram_functions n).mor h_refl) begin fapply Lhom.on_function, exact @mor D F i j H, end) x = (F.mor H).on_function x,
+   have := Lhom.comp_on_function' (F.mor h_refl) (F.mor H) n, rw[<-this,<-F.h_mor]},
+  {  refine ⟨j,(F.mor H).on_relation x, H, h_refl, rfl, _⟩,
+    change (function.comp ((diagram_relations n).mor h_refl) begin fapply Lhom.on_relation, exact @mor D F i j H, end) x = (F.mor H).on_relation x,
+   have := Lhom.comp_on_relation' (F.mor h_refl) (F.mor H) n, rw[<-this,<-F.h_mor]}
+end
+
+/- Given a cocone V over a diagram D, return the canonical map colim D → V-/
+def universal_map_language {D} {F : directed_diagram_language D} {V : cocone_language F} : colimit_language F →ᴸ (V.vertex) :=
+begin
+  split, all_goals{intro n,
+  fapply quotient.lift},
+
+{exact λp, begin fapply @Lhom.on_function, exact F.obj p.fst, exact @map D F V p.fst, exact p.snd end},
+  {intros p q H, rcases p with ⟨i,x⟩, rcases q with ⟨j,y⟩, simp only *,
+   simp only [(≈), germ_relation] at H,
+   rcases H with ⟨k,z,f1, f2, H1, H2⟩,
+   change (V.map i).on_function x = (V.map j).on_function y, have : (V.map i).on_function x = (V.map k).on_function ((F.mor f1).on_function x),
+   simp only [V.h_compat f1, eq_self_iff_true, function.comp_app],
+   have : (V.map j).on_function y = (V.map k).on_function ((F.mor f2).on_function y),
+   simp only [V.h_compat f2, eq_self_iff_true, function.comp_app],
+   simp only [*, eq_self_iff_true]},
+
+{exact λp, begin fapply @Lhom.on_relation, exact F.obj p.fst, exact @map D F V p.fst, exact p.snd end},
+  {intros p q H, rcases p with ⟨i,x⟩, rcases q with ⟨j,y⟩, simp only *,
+   simp only [(≈), germ_relation] at H, rcases H with ⟨k,z,f1,f2,H1,H2⟩,
+   change (V.map i).on_relation x = (V.map j).on_relation y, have : (V.map i).on_relation x = (V.map k).on_relation ((F.mor f1).on_relation x),
+   simp only [V.h_compat f1, eq_self_iff_true, function.comp_app],
+   have : (V.map j).on_relation y = (V.map k).on_relation ((F.mor f2).on_relation y),
+   simp only [V.h_compat f2, eq_self_iff_true, function.comp_app],
+   simp only [*, eq_self_iff_true]},
+end
+
+namespace omega_colimit_language
+/- Facts about directed colimits indexed by ℕ'. -/
+def diagram.mk.map {F : ℕ → Language} {h_succ : ∀{i : ℕ}, F i →ᴸ F (i+1)} : Π (x y : ℕ), x ≤ y → (F x →ᴸ F y)
+| x 0 h := by {rw[nat.eq_zero_of_le_zero h], exact ⟨λn, id, λn, id⟩}
+| x (y+1) h := by {by_cases x = y + 1, rw[h], exact ⟨λn, id, λn, id⟩, refine h_succ ∘  _,
+                  apply diagram.mk.map, apply nat.le_of_le_and_ne_succ, repeat{assumption}}
+
+--TODO(jesse) finish converting this to language versions and refactor henkin_language_chain
+-- @[simp]lemma diagram.mk.map_self_id {F : ℕ → Type*} {h_succ : ∀(i : ℕ), F i → F (i+1)} (x : ℕ) :
+--                   @diagram.mk.map F @h_succ x x (by constructor) = id :=
+-- by {induction x, tidy, simp[diagram.mk.map,*], refl}
+
+
+-- /- If the successive maps of h_succ are injective, then all their compositions are injective -/
+-- lemma diagram.mk.map_inj {F : ℕ → Type*} {h_succ : ∀(i : ℕ), F i → F (i+1)} {h_inj : ∀ {i : ℕ}, function.injective (@h_succ i )} (x y : ℕ) (h : x ≤ y) : function.injective (@diagram.mk.map F h_succ x y h) :=
+-- begin
+--   induction y,
+--     {have : x = 0, by exact nat.eq_zero_of_le_zero h, dsimp[*,diagram.mk.map], finish},
+--     by_cases x = y_n + 1,
+--       {dsimp[*, diagram.mk.map], finish},
+--     have : x ≤ y_n, by {apply nat.le_of_le_and_ne_succ, repeat{assumption}},
+--     simp[*, diagram.mk.map], apply function.injective_comp, apply h_inj, apply y_ih
+-- end
+
+-- -- /- Given a ℕ-indexed family of types and a way of assigning maps between successive objects
+-- --    in this family, return the induced directed_diagram over ℕ'. -/
+-- def diagram.mk(F : ℕ → Type*) (h_succ :∀{i : ℕ}, F i → F (i+1)) : directed_diagram ℕ' :=
+-- begin
+-- refine ⟨F, by {apply diagram.mk.map, assumption}, _⟩,
+--   intros x y z H1 H2 H3,
+--     induction z, induction y, induction x,
+--     dsimp[diagram.mk.map], refl,
+--      by {exfalso, fapply nat.succ_ne_zero, exact x_n, apply (nat.le_zero_iff).mp, assumption},
+--      by {exfalso, fapply nat.succ_ne_zero, exact y_n, apply (nat.le_zero_iff).mp, assumption},
+--      by_cases y = z_n+1, subst h;
+--        by_cases x = z_n+1;
+--        {repeat{dsimp[diagram.mk.map], simp*, refl}},
+--      by_cases x = z_n+1,
+--        {exfalso, have : y < z_n+1, by {fapply nat.lt_of_le_and_ne,
+--          repeat{assumption}}, dsimp at *, linarith},
+--        {have h_x : x ≤ z_n; have h_y : y ≤ z_n,
+--          all_goals{try{apply nat.le_of_le_and_ne_succ, repeat{assumption}}},
+--         have := @z_ih h_y h_x,
+--         dsimp[diagram.mk.map], dedup,
+--         simp only [h, h_1, dif_neg, not_false_iff, colimit.nat.le_of_le_and_ne_succ],
+--         rw[this]}
+-- end
+
+
+end omega_colimit_language
+
+end colimit
+
+open colimit
+
+open omega_colimit
+
+/- The Henkin construction consists of the following:
+   1. Constructing a ℕ-indexed chain of languages and theories, and
+   2. Taking the union of that chain. -/
+
+/- To define henkin_language_step, there is an inductive type of new function
+   function symbols, comprising an inclusion constructor for the symbols
+   from L, and a witness constructor which introduces witnesses for every
+   bounded_formula 1-/
+inductive henkin_language_functions (L : Language.{u}) : ℕ → Type u
+  | inc : ∀ {n}, L.functions n → henkin_language_functions n
+  | wit : bounded_formula L 1 → henkin_language_functions 0
+
+open henkin_language_functions
+
+/- The basic step of the Henkin construction on languages.
+   Given a language L, return a language L' with constants
+   witnessing all bounded_formula 1-/
+@[reducible]def henkin_language_step (L : Language.{u}) : Language.{u} :=
+  ⟨henkin_language_functions L, L.relations⟩
+
+def wit' {L : Language} : bounded_formula L 1 → (henkin_language_step L).constants := wit
+
+def henkin_language_inclusion {L : Language} : L →ᴸ henkin_language_step L :=
+  ⟨λ n f, inc f, λn, id⟩
+
+lemma henkin_language_inclusion_inj {L : Language} : Lhom.is_injective (@henkin_language_inclusion L) :=
+begin
+  split, all_goals{intro n, intros x y H, try{exact H}},
+  fapply @henkin_language_functions.inc.inj_arrow,
+  exact L, exact n, exact x, exact y, exact H, simp only [imp_self]
+end
+
+/- The basic step of the Henkin construction on theories.
+   Given an L-theory T, return an L'-theory T' which is T expanded by
+   sentences saying that the new witnesses are witnesses. -/
+@[reducible]def wit_property {L : Language} (f : bounded_formula L 1) (c : L.constants) :
+  sentence L :=
+(∃'f) ⟹ f[bd_const c/0]
+
+open fol.Lhom
+def henkin_theory_step {L} (T : Theory L) : Theory $ henkin_language_step L :=
+Theory_induced henkin_language_inclusion T ∪
+(λ f : bounded_formula L 1,
+  wit_property (henkin_language_inclusion.on_bounded_formula f) (wit' f)) '' (set.univ : set $ bounded_formula L 1)
+
+lemma is_consistent_henkin_theory_step {L} {T : Theory L} (hT : is_consistent T) :
+  is_consistent (henkin_theory_step T) :=
+begin
+  refine eq.mp _ (is_consistent_extend hT henkin_language_inclusion_inj
+    (λf, (∃' f).cast1 ⟹ f) _ wit _ _),
+  {
+    congr1, congr1, apply set.image_congr', intro f, ext,
+    simp only [wit_property, wit'],
+    simp only [on_bounded_formula],
+    simp only [subst0_bounded_formula_imp],
+    simp only [fst_imp],
+    simp only [and_true, eq_self_iff_true],
+    rw [on_bounded_formula_ex, on_bounded_formula_cast1, subst0_bounded_formula],
+    simp only [fol.bounded_preformula.cast_eq_fst,
+      subst_bounded_formula_fst, fst_ex, fol.bounded_preformula.cast1_fst],
+    rw subst_sentence_irrel,
+  },
+  { intro f, apply falsumE, apply impE (∃' f.fst),
+    { apply impI, apply impE _ axm2, apply exE axm1,
+      apply exI &0, rw [lift_subst_formula_cancel], apply impI axm2 },
+    { apply falsumE, apply impE _ axm2, apply exI &0,
+      apply impI, apply exfalso, apply impE _ axm2,
+        rw [bounded_preformula.cast1_fst, subst_sentence_irrel], exact axm1 }},
+  { intros f f' h, cases h, refl },
+  { intro f, intro h, rcases h with ⟨f', hf'⟩, cases hf' }
+end
+
+@[reducible]def henkin_language_chain_objects {L : Language} : ℕ → Language
+  | 0 := L
+  | (n+1) := henkin_language_step (henkin_language_chain_objects n)
+
+@[simp]lemma obvious {L : Language} {i : ℕ} : henkin_language_functions (@henkin_language_chain_objects L i) 0 = (@henkin_language_chain_objects L (i+1)).constants :=
+by refl
+
+local infix ` ∘ `:60 := Lhom.comp
+
+def henkin_language_chain_maps (L : Language) :
+  Π {x y : ℕ}, x ≤ y →
+  (@henkin_language_chain_objects L x →ᴸ @henkin_language_chain_objects L y)
+| 0     0 h := Lhom.id L
+| (x+1) 0 h := false.elim (nat.not_succ_le_zero _ h)
+| 0 (y+1) h :=
+@henkin_language_inclusion (@henkin_language_chain_objects L y)
+    ∘
+    (henkin_language_chain_maps (nat.zero_le _))
+| (x+1) (y+1) h := dite (x + 1 = y + 1)
+  (λ heq, cast1 (by rw heq))
+  (λ hneq,
+    @henkin_language_inclusion (@henkin_language_chain_objects L y)
+    ∘
+    (henkin_language_chain_maps (nat.le_of_le_and_ne_succ h hneq)))
+
+-- def henkin_language_chain_maps' (L : Language): Π x y, x ≤ y →
+--   (@henkin_language_chain_objects L x →ᴸ @henkin_language_chain_objects L y)
+-- | x 0 H := by {have : x = 0, by exact nat.eq_zero_of_le_zero H, rw[this], apply Lhom.id}
+-- | x (y+1) H := by {by_cases x = y + 1, rw[h], fapply Lhom.id,
+--                refine @henkin_language_inclusion (@henkin_language_chain_objects L y) ∘ _,
+--                fapply henkin_language_chain_maps,
+--                fapply nat.le_of_le_and_ne_succ, exacts [H, h]}
+
+lemma henkin_language_chain_maps_inj (L : Language) :
+  Π {i j : ℕ}, Π (h : i ≤ j),
+  Lhom.is_injective (henkin_language_chain_maps L h)
+| 0     0 h := ⟨ λ n x y H, H , λ n x y H, H ⟩
+| (i+1) 0 h := false.elim (nat.not_succ_le_zero _ h)
+| 0 (j+1) h :=
+begin
+  fsplit,
+  {
+    intro n,
+    apply function.injective.comp,
+    {fapply henkin_language_inclusion_inj.on_function},
+    {
+      intros a b H,
+      have hind := (henkin_language_chain_maps_inj (_)).on_function,
+      apply hind,
+      exact H,
+    },
+  },
+  {
+    intro n,
+    apply function.injective.comp,
+    {fapply henkin_language_inclusion_inj.on_relation},
+    {
+      intros a b H,
+      have hind := (henkin_language_chain_maps_inj (_)).on_relation,
+      apply hind,
+      exact H,
+    },
+  },
+end
+| (i+1) (j+1) h :=
+begin
+  unfold henkin_language_chain_maps,
+  by_cases hij : i + 1 = (j + 1),
+  {
+    simp only [hij, dif_pos], fsplit,
+    {intro n, exact λ _ _, (cast_inj _).mp,},
+    {intro n, exact λ _ _, (cast_inj _).mp,},
+  },
+  {
+    simp only [hij, dif_neg, not_false_iff], fsplit,
+    {
+      intro n,
+      apply function.injective.comp,
+      {fapply henkin_language_inclusion_inj.on_function},
+      {
+        intros a b H,
+        have hind := (henkin_language_chain_maps_inj (_)).on_function,
+        apply hind,
+        exact H,
+      },
+    },
+    {
+      intro n,
+      apply function.injective.comp,
+      {fapply henkin_language_inclusion_inj.on_relation},
+      {
+        intros a b H,
+        have hind := (henkin_language_chain_maps_inj (_)).on_relation,
+        apply hind,
+        exact H,
+      },
+    },
+  }
+end
+
+lemma cast_comp_eq_self {L L1 : Language} {ϕ : L1 →ᴸ L} :
+  {on_function := λ (n : ℕ), cast rfl, on_relation := λ (n : ℕ), cast rfl} ∘ ϕ
+  = ϕ :=
+by cases ϕ; refl
+
+/- Given a language, iterate henkin_language_step, returning this data in the form
+   of a directed diagram of types indexed by ℕ' -/
+def henkin_language_chain {L : Language} :
+  directed_diagram_language directed_type_of_nat :=
+⟨ @henkin_language_chain_objects L ,
+  λ x y H, henkin_language_chain_maps _ H ,
+  λ x y z Hxy Hyz Hxz,
+  begin
+    induction z with z hz,
+    {
+      induction y with y hy, induction x with x hx,
+      {dsimp[diagram.mk.map], refl},
+      {by {exfalso, fapply nat.succ_ne_zero, exact x, apply (nat.le_zero_iff).mp, assumption}},
+      {by {exfalso, fapply nat.succ_ne_zero, exact y, apply (nat.le_zero_iff).mp, assumption}},
+    },
+    {
+      by_cases hyz : y = z+1,
+      {
+        subst hyz,
+        simp only [henkin_language_chain_maps, dif_pos],
+        rw trivial_cast1_is_left_identity,
+      },
+      {
+        by_cases hxz : x = z+1,
+        { exfalso, apply nat.le_lt_antisymm Hxy,
+          subst hxz, exact nat.lt_of_le_and_ne Hyz hyz,
+        },
+        { have hind := hz (nat.le_of_le_and_ne_succ Hyz hyz)
+            (nat.le_of_le_and_ne_succ Hxz hxz),
+          induction y with y hy,
+          {
+            induction x with x hx,
+            { simp only [henkin_language_chain_maps, id_is_right_identity] },
+            { exfalso, exact nat.not_succ_le_zero _ Hxy, }
+          },
+          { induction x with x hx,
+            { simp only [henkin_language_chain_maps, dif_neg hyz, hind] },
+            { simpa only [henkin_language_chain_maps, dif_neg hyz,
+                dif_neg hxz, hind] }, },
+        },
+      },
+    },
+  end ⟩
+
+@[simp]lemma id_of_self_map (L : Language) : ∀ k : ℕ,
+  (henkin_language_chain_maps L (le_refl k)) =
+  Lhom.id ((@henkin_language_chain L).obj k)
+| 0 := by refl
+| (n+1) := by {dsimp[henkin_language_chain_maps], simpa }
+
+@[simp]lemma henkin_language_inclusion_chain_map {i} {L : Language} :
+  henkin_language_inclusion =
+  @henkin_language_chain_maps L i (i + 1) (by simp[nat.le_succ]) :=
+begin
+  induction i with i hi,
+  { simp only [henkin_language_chain_maps],
+    exact symm id_is_right_identity },
+  {
+    have hne : i + 1 ≠ i.succ + 1 := by simp,
+    simp only [henkin_language_chain_maps, dif_neg hne, dif_pos],
+    exact symm trivial_cast1_is_right_identity,
+    },
+end
+
+def L_infty (L) : Language :=
+   colimit_language $ @henkin_language_chain L
+
+/-- For every n : ℕ, return the canonical inclusion L_n → L_infty  --/
+def henkin_language_canonical_map {L : Language} (m : ℕ) : (@henkin_language_chain L).obj m →ᴸ (@L_infty L) := by apply canonical_map_language
+
+@[simp]lemma henkin_language_canonical_map_inj {L : Language} (m : ℕ) : Lhom.is_injective $ @henkin_language_canonical_map L m :=
+begin
+  split,
+
+  {intro n, unfold henkin_language_canonical_map canonical_map_language Lhom.on_function,
+  have := @canonical_map_inj_of_transition_maps_inj directed_type_of_nat (@diagram_functions directed_type_of_nat (@henkin_language_chain L) n), unfold canonical_map at this, apply this,intros i j H, dsimp[diagram_functions, henkin_language_chain],
+  fapply ((henkin_language_chain_maps_inj) L H).on_function},
+
+  {intro n, unfold henkin_language_canonical_map canonical_map_language Lhom.on_relation,
+  have := @canonical_map_inj_of_transition_maps_inj directed_type_of_nat (@diagram_relations directed_type_of_nat (@henkin_language_chain L) n), unfold canonical_map at this, apply this,intros i j H, dsimp[diagram_relations, henkin_language_chain],
+  fapply ((henkin_language_chain_maps_inj) L H).on_relation}
+end
+
+/- To prove that T_infty is Henkin, we'll have to exhibit a witnessing function of the form
+  wit : bounded_formula 1 → L_infty.constants.
+
+  To do this, we have to recursively go through formulas and terms and show that for every
+  formula, there exists some N such that all the symbols in that formula were contained in L_N,
+  and therefore, the wit function for L_N introduces the constant we want.
+
+  The natural way to proceed is to define the induced colimit on bounded_formulas, etc.
+
+  Then, we can define the required wit function by taking a bounded formula, picking a
+  representative from stage N, applying the wit function from stage N to get something in
+  stage N+1, and then pushing it up to L_infty. -/
+
+/- In what follows, "l" is always pre(whatever) level, "k" is always chain index,
+   and "n" is always the bound in bounded_(whatever)-/
+
+def henkin_term_chain {L : Language} (l : ℕ) : directed_diagram ℕ' :=
+begin
+  refine ⟨λ k, preterm (@henkin_language_chain_objects L k) l, _, _⟩,
+  {intros x y H, apply Lhom.on_term, apply @henkin_language_chain_maps L, exact H},
+  {intros x y z f1 f2 f3, dsimp only [*],
+   have : (henkin_language_chain_maps L f3) =
+   (henkin_language_chain_maps L f2) ∘ (henkin_language_chain_maps L f1),
+   fapply henkin_language_chain.h_mor, simp*}
+end
+
+def henkin_formula_chain {L : Language} (l : ℕ) : directed_diagram ℕ' :=
+begin
+  refine ⟨λ k, preformula (@henkin_language_chain_objects L k) l, _, _⟩,
+  {intros x y H, apply Lhom.on_formula, apply @henkin_language_chain_maps L, exact H},
+  {intros x y z f1 f2 f3, dsimp only [*],
+   have : (henkin_language_chain_maps L f3) =
+   (henkin_language_chain_maps L f2) ∘ (henkin_language_chain_maps L f1),
+   fapply henkin_language_chain.h_mor, simp*}
+end
+
+def henkin_bounded_term_chain {L : Language} (n l : ℕ) : directed_diagram ℕ' :=
+begin
+  refine ⟨λ k, bounded_preterm (@henkin_language_chain_objects L k) n l, _, _⟩,
+  {intros x y H, apply Lhom.on_bounded_term, apply @henkin_language_chain_maps L, exact H},
+  {intros x y z f1 f2 f3, dsimp only [*],
+   have : (henkin_language_chain_maps L f3) =
+   (henkin_language_chain_maps L f2) ∘ (henkin_language_chain_maps L f1),
+   fapply henkin_language_chain.h_mor, rw[this, Lhom.comp_on_bounded_term]}
+end
+
+@[reducible] def henkin_bounded_term_chain' {L : Language} : directed_diagram ℕ' := @henkin_bounded_term_chain L 1 0
+
+def henkin_bounded_formula_chain {L : Language} (n l : ℕ) : directed_diagram ℕ' :=
+begin
+  refine ⟨λ k, bounded_preformula (@henkin_language_chain_objects L k) n l, _, _⟩,
+  {intros x y H, apply Lhom.on_bounded_formula, apply @henkin_language_chain_maps L, exact H},
+  {intros x y z f1 f2 f3, dsimp only [*],
+   have : (henkin_language_chain_maps L f3) =
+   (henkin_language_chain_maps L f2) ∘ (henkin_language_chain_maps L f1),
+   fapply henkin_language_chain.h_mor, rw[this, Lhom.comp_on_bounded_formula]}
+end
+
+@[reducible]def henkin_bounded_formula_chain' {L : Language} : directed_diagram ℕ' := @henkin_bounded_formula_chain L 1 0
+
+/- L_infty := colim L_n is naturally a cocone over the diagram of languages -/
+def cocone_of_L_infty {L : Language} : cocone_language (@henkin_language_chain L) :=
+  cocone_of_colimit_language _
+
+def cocone_of_term_L_infty {L : Language } (l : ℕ) : cocone (@henkin_term_chain L l) :=
+begin
+  refine ⟨preterm (L_infty L) l,_,_⟩,
+  {intro i, fapply Lhom.on_term, fapply henkin_language_canonical_map},
+  {intros i j H, dsimp[henkin_term_chain],
+  rw[<-Lhom.comp_on_term],
+  have : henkin_language_canonical_map i = (henkin_language_canonical_map j ∘ henkin_language_chain_maps L H), swap, rw[this],
+  unfold henkin_language_canonical_map,
+  exact (@cocone_of_L_infty L).h_compat _,}
+end
+
+def cocone_of_formula_L_infty {L : Language } (l : ℕ) : cocone (@henkin_formula_chain L l) :=
+begin
+  refine ⟨preformula (L_infty L) l,_,_⟩,
+  {intro i, fapply Lhom.on_formula, fapply henkin_language_canonical_map},
+  {intros i j H, dsimp[henkin_formula_chain],
+  rw[<-Lhom.comp_on_formula],
+  have : henkin_language_canonical_map i = (henkin_language_canonical_map j ∘ henkin_language_chain_maps L H), swap, rw[this],
+  unfold henkin_language_canonical_map,
+  exact (@cocone_of_L_infty L).h_compat _,}
+end
+
+def cocone_of_bounded_term_L_infty {L : Language } (n l : ℕ) : cocone (@henkin_bounded_term_chain L n l) :=
+begin
+  refine ⟨bounded_preterm (L_infty L) n l,_,_⟩,
+  {intro i, fapply Lhom.on_bounded_term, fapply henkin_language_canonical_map},
+  {intros i j H, dsimp[henkin_bounded_term_chain],
+  rw[<-Lhom.comp_on_bounded_term],
+  have : henkin_language_canonical_map i = (henkin_language_canonical_map j ∘ henkin_language_chain_maps L H), swap, rw[this],
+  unfold henkin_language_canonical_map,
+  exact (@cocone_of_L_infty L).h_compat _,}
+end
+
+def cocone_of_bounded_formula_L_infty {L : Language } (n l : ℕ) : cocone (@henkin_bounded_formula_chain L n l) :=
+begin
+  refine ⟨bounded_preformula (L_infty L) n l,_,_⟩,
+  {intro i, fapply Lhom.on_bounded_formula, fapply henkin_language_canonical_map},
+  {intros i j H, dsimp[henkin_bounded_formula_chain],
+  rw[<-Lhom.comp_on_bounded_formula],
+  have : henkin_language_canonical_map i = (henkin_language_canonical_map j ∘ henkin_language_chain_maps L H), swap, rw[this],
+  unfold henkin_language_canonical_map,
+  exact (@cocone_of_L_infty L).h_compat _,}
+end
+
+/- bounded_formula (L_infty L) 1 is naturally a cocone over the diagram of bounded_formulas -/
+def cocone_of_bounded_formula'_L_infty {L : Language} : cocone (@henkin_bounded_formula_chain' L) :=
+begin
+  refine ⟨bounded_formula (L_infty L) 1,_,_⟩,
+  {intro i, fapply Lhom.on_bounded_formula, fapply henkin_language_canonical_map},
+  {intros i j H, dsimp[henkin_bounded_formula_chain', henkin_bounded_formula_chain],
+  rw[<-Lhom.comp_on_bounded_formula],
+  have : henkin_language_canonical_map i = (henkin_language_canonical_map j ∘ henkin_language_chain_maps L H), swap, rw[this],
+  unfold henkin_language_canonical_map,
+  exact (@cocone_of_L_infty L).h_compat _,}
+end
+
+def term_comparison {L : Language} (l) : colimit (@henkin_term_chain L l) → preterm (L_infty L) l :=
+begin
+  change colimit (@henkin_term_chain L l)  → (@cocone_of_term_L_infty L l).vertex,
+  apply colimit.universal_map
+end
+
+def formula_comparison {L : Language} (l) : colimit (@henkin_formula_chain L l) → preformula (L_infty L) l :=
+begin
+  change colimit (@henkin_formula_chain L l)  → (@cocone_of_formula_L_infty L l).vertex,
+  apply colimit.universal_map
+end
+
+def bounded_term_comparison {L : Language} (n l) : colimit (@henkin_bounded_term_chain L n l) → bounded_preterm (L_infty L) n l :=
+begin
+  change colimit (@henkin_bounded_term_chain L n l)  → (@cocone_of_bounded_term_L_infty L n l).vertex,
+  apply colimit.universal_map
+end
+
+@[reducible]def bounded_term'_comparison {L : Language}  : colimit (@henkin_bounded_term_chain' L) → bounded_term (L_infty L) 1 := @bounded_term_comparison L 1 0
+
+def bounded_formula_comparison {L : Language} (n l) : colimit (@henkin_bounded_formula_chain L n l) → bounded_preformula (L_infty L) n l :=
+begin
+  change colimit (@henkin_bounded_formula_chain L n l)  → (@cocone_of_bounded_formula_L_infty L n l).vertex,
+  apply colimit.universal_map
+end
+
+@[reducible]def bounded_formula'_comparison {L : Language} : colimit (@henkin_bounded_formula_chain' L) → bounded_formula (L_infty L) 1 := @bounded_formula_comparison L 1 0
+
+-- to proceed, need to show that bounded_formula_comparison, as we've defined it,
+-- commutes with operations on bounded formulas -- so we need to generalize from
+-- bounded_formula 1 to bounded_formula n, and prove colimit statements for terms, etc
+-- to complete the structural recursion
+/- The universal map from colimit preterm L_n → preterm L_infty is a bijection -/
+-- TODO(jesse) refactor with new colimit lemmas
+lemma term_comparison_bijective {L : Language} (l) : function.bijective (@term_comparison L l) :=
+begin
+  refine ⟨_,_⟩,
+  {{unfold term_comparison id, fapply universal_map_inj_of_components_inj,
+  change ∀ i : ℕ, function.injective ((cocone_of_term_L_infty l).map i),
+  dsimp[cocone_of_term_L_infty],  intro m,
+  fapply Lhom.on_term_inj (@henkin_language_canonical_map_inj L m)},},
+  {intro f, induction f,
+    {refine ⟨(by {fapply canonical_map, by {change ℕ, exact 0}, exact var f}), by split⟩},
+    {have W := germ_rep f_f, rcases W with ⟨⟨i,x⟩, Hx⟩, fapply exists.intro,
+     fapply canonical_map i, fapply func, exact x, rw[<-Hx], refl},
+    {rcases f_ih_t with ⟨t, Ht⟩, rcases f_ih_s with ⟨s,Hs⟩, have Wt := germ_rep t,
+    have Ws := germ_rep s, rcases Wt with ⟨⟨i,x_t⟩, Hxt⟩, rcases Ws with ⟨⟨j, x_s⟩, Hxs⟩,
+    let x_t' : (henkin_term_chain (f_l + 1)).obj (i+j),
+      fapply (henkin_term_chain (f_l + 1)).mor, exact i,
+      simp only [ℕ', directed_type.rel, id.def, zero_le, le_add_iff_nonneg_right],
+      exact x_t,
+    let x_s' : (henkin_term_chain 0).obj (i+j),
+      fapply (henkin_term_chain 0).mor, exact j,
+      simp only [ℕ', directed_type.rel, zero_le, le_add_iff_nonneg_left],
+      exact x_s,
+    have Hxt' : ⟦(⟨i+j,x_t'⟩ : coproduct_of_directed_diagram $
+      henkin_term_chain (f_l + 1))⟧ = t,
+    {
+      rw[<-Hxt],
+      rw quotient.eq,
+      simp only [(≈), germ_relation],
+      refine ⟨(i+j),x_t', nat.le_of_eq rfl , nat.le_add_right _ _ , _ ⟩,
+      dsimp[henkin_term_chain, henkin_language_chain_maps],
+      simp only [id_of_self_map], split,
+      {exact Lhom.id_term _ _},
+      {refl},
+    },
+    have Hxs' : ⟦(⟨i+j,x_s'⟩ : coproduct_of_directed_diagram $
+      henkin_term_chain 0)⟧ = s,
+    {
+      rw[<-Hxs],
+      rw quotient.eq,
+      simp only [(≈), germ_relation],
+      refine ⟨(i+j),x_s', nat.le_of_eq rfl , nat.le_add_left _ _ , _ ⟩,
+      dsimp[henkin_term_chain, henkin_language_chain_maps],
+      simp only [id_of_self_map], split,
+      {exact Lhom.id_term _ _},
+      {refl},
+    },
+    fapply exists.intro, fapply canonical_map, change ℕ, exact (i + j),
+    fapply app, exact x_t', exact x_s', rw[<-Ht, <-Hs, <-Hxt', <-Hxs'], refl
+    },},
+end
+
+/- At some point, I should write out explicitly the fact that all the comparison maps
+   structurally recurse -/
+lemma formula_comparison_bijective {L : Language} (l) : function.bijective (@formula_comparison L l) :=
+begin
+  refine ⟨_,_⟩,
+  {{unfold formula_comparison id, fapply universal_map_inj_of_components_inj,
+  change ∀ i : ℕ, function.injective ((cocone_of_formula_L_infty l).map i),
+  dsimp[cocone_of_formula_L_infty],  intro m,
+  fapply Lhom.on_formula_inj (@henkin_language_canonical_map_inj L m)},},
+  {intro f, induction f,
+  {refine ⟨(by {fapply canonical_map, by {change ℕ, exact 0}, exact falsum}), by split⟩},
+  {
+    rcases (term_comparison_bijective 0).right f_t₁ with ⟨t₁, H₁⟩, rcases (term_comparison_bijective 0).right f_t₂ with ⟨t₂, H₂⟩,
+    rcases germ_rep t₁ with ⟨⟨i,x⟩,Hx⟩, rcases germ_rep t₂ with ⟨⟨j,y⟩,Hy⟩,
+    fapply exists.intro, fapply canonical_map, exact i+j, fapply equal,
+    exact push_to_sum_r x j, exact push_to_sum_l y i,
+    rw[<-H₁, <-H₂,<-Hx, <-Hy, <-canonical_map_quotient, same_fiber_as_push_to_r x j ,<-canonical_map_quotient, same_fiber_as_push_to_l y i],
+    simpa only},
+  {have x := germ_rep f_R, rcases x with ⟨⟨i,x⟩,H⟩, fapply exists.intro, have R' := rel x,
+   exact ⟦⟨i,R'⟩⟧, tidy},
+  {rcases f_ih with ⟨t₁, H₁⟩,
+   rcases (term_comparison_bijective 0).right f_t with ⟨t₂, H₂⟩,
+   rcases germ_rep t₁ with ⟨⟨i,x⟩,Hx⟩, rcases germ_rep t₂ with ⟨⟨j,y⟩,Hy⟩,
+   fapply exists.intro, fapply canonical_map, exact i+j, fapply apprel,
+   exact push_to_sum_r x j, exact push_to_sum_l y i,
+    rw[<-H₁, <-H₂,<-Hx, <-Hy, <-canonical_map_quotient, same_fiber_as_push_to_r x j ,<-canonical_map_quotient, same_fiber_as_push_to_l y i],
+    simpa only},
+  {rcases f_ih_f₁ with ⟨t₁, H₁⟩, rcases f_ih_f₂ with ⟨t₂, H₂⟩,
+   rcases germ_rep t₁ with ⟨⟨i,x⟩,Hx⟩, rcases germ_rep t₂ with ⟨⟨j,y⟩,Hy⟩,
+   fapply exists.intro, fapply canonical_map, exact (i+j), fapply imp,
+   exact push_to_sum_r x j, exact push_to_sum_l y i,
+    rw[<-H₁, <-H₂,<-Hx, <-Hy, <-canonical_map_quotient, same_fiber_as_push_to_r x j ,<-canonical_map_quotient, same_fiber_as_push_to_l y i],
+    simpa only},
+  {rcases f_ih with ⟨t₁, H₁⟩,
+   rcases germ_rep t₁ with ⟨⟨i,x⟩,Hx⟩,
+   fapply exists.intro, fapply canonical_map, exact i, fapply all,
+   exact x, rw[<-H₁, <-Hx], simpa only}}
+end
+
+@[simp]lemma bounded_term_comparison_bijective {L : Language} (n l) : function.bijective (@bounded_term_comparison L n l) :=
+begin
+refine ⟨_,_⟩,
+  {{unfold bounded_term_comparison id, fapply universal_map_inj_of_components_inj,
+  change ∀ i : ℕ, function.injective ((cocone_of_bounded_term_L_infty n l).map i),
+  dsimp[cocone_of_bounded_term_L_infty],  intro m,
+  fapply Lhom.on_bounded_term_inj (@henkin_language_canonical_map_inj L m)},},
+  {
+    intro f, induction f,
+    {refine ⟨(by {fapply canonical_map, by {change ℕ, exact 0}, exact bd_var f}), by split⟩},
+    {have W := germ_rep f_f, rcases W with ⟨⟨i,x⟩, Hx⟩, fapply exists.intro,
+      fapply canonical_map i, fapply bd_func, exact x, rw[<-Hx], refl,},
+    {rcases f_ih_t with ⟨t, Ht⟩, rcases f_ih_s with ⟨s,Hs⟩, have Wt := germ_rep t,
+    have Ws := germ_rep s, rcases Wt with ⟨⟨i,x_t⟩, Hxt⟩, rcases Ws with ⟨⟨j, x_s⟩, Hxs⟩,
+    let x_t' : (henkin_bounded_term_chain n (f_l + 1)).obj (i+j),
+      fapply (henkin_bounded_term_chain n (f_l + 1)).mor, exact i,
+      simp only [ℕ', directed_type.rel, id.def, zero_le, le_add_iff_nonneg_right],
+      exact x_t,
+    let x_s' : (henkin_bounded_term_chain n 0).obj (i+j),
+      fapply (henkin_bounded_term_chain n 0).mor, exact j,
+      simp only [ℕ', directed_type.rel, zero_le, le_add_iff_nonneg_left],
+      exact x_s,
+    have Hxt' : ⟦(⟨i+j,x_t'⟩ : coproduct_of_directed_diagram $ henkin_bounded_term_chain n (f_l + 1))⟧ = t,
+    {
+      rw[<-Hxt],
+      rw quotient.eq,
+      simp only [(≈), germ_relation],
+      refine ⟨(i+j),x_t', nat.le_of_eq rfl , nat.le_add_right _ _ , _ ⟩,
+      dsimp[henkin_bounded_term_chain, henkin_language_chain_maps],
+      simp only [id_of_self_map], split,
+      {exact Lhom.id_bounded_term _ _ _},
+      {refl},
+    },
+    have Hxs' : ⟦(⟨i+j,x_s'⟩ : coproduct_of_directed_diagram $ henkin_bounded_term_chain n 0)⟧ = s,
+    {
+      rw[<-Hxs],
+      rw quotient.eq,
+      simp only [(≈), germ_relation],
+      refine ⟨(i+j),x_s', nat.le_of_eq rfl , nat.le_add_left _ _ , _ ⟩,
+      dsimp[henkin_bounded_term_chain, henkin_language_chain_maps],
+      simp only [id_of_self_map], split,
+      {exact Lhom.id_bounded_term _ _ _},
+      {refl},
+    },
+    fapply exists.intro, fapply canonical_map, change ℕ, exact (i + j),
+    fapply bd_app, exact x_t', exact x_s', rw[<-Ht, <-Hs, <-Hxt', <-Hxs'], refl},}
+end
+
+@[simp]lemma bounded_formula_comparison_bijective {L : Language} (n l) : function.bijective (@bounded_formula_comparison L n l) :=
+begin
+refine ⟨_,_⟩,
+  {{unfold bounded_formula_comparison id, fapply universal_map_inj_of_components_inj,
+  change ∀ i : ℕ, function.injective ((cocone_of_bounded_formula_L_infty n l).map i),
+  dsimp[cocone_of_bounded_formula_L_infty],  intro m,
+  fapply Lhom.on_bounded_formula_inj (@henkin_language_canonical_map_inj L m)},},
+  {intro f, induction f,
+  {refine ⟨(by {fapply canonical_map, by {change ℕ, exact 0}, exact bd_falsum}), by split⟩},
+  {
+    rcases (bounded_term_comparison_bijective f_n 0).right f_t₁ with ⟨t₁, H₁⟩, rcases (bounded_term_comparison_bijective f_n 0).right f_t₂ with ⟨t₂, H₂⟩,
+    rcases germ_rep t₁ with ⟨⟨i,x⟩,Hx⟩, rcases germ_rep t₂ with ⟨⟨j,y⟩,Hy⟩,
+    fapply exists.intro, fapply canonical_map, exact i+j, fapply bd_equal,
+    exact push_to_sum_r x j, exact push_to_sum_l y i,
+    -- simp[H₁, H₂],
+    rw[<-H₁, <-H₂,<-Hx, <-Hy, <-canonical_map_quotient, same_fiber_as_push_to_r x j ,<-canonical_map_quotient, same_fiber_as_push_to_l y i],
+    simpa only},
+  {have x := germ_rep f_R, rcases x with ⟨⟨i,x⟩,H⟩, fapply exists.intro, have R' := bd_rel x,
+   exact ⟦⟨i,R'⟩⟧, tidy},
+  {rcases f_ih with ⟨t₁, H₁⟩,
+   rcases (bounded_term_comparison_bijective _ 0).right f_t with ⟨t₂, H₂⟩,
+   rcases germ_rep t₁ with ⟨⟨i,x⟩,Hx⟩, rcases germ_rep t₂ with ⟨⟨j,y⟩,Hy⟩,
+   fapply exists.intro, fapply canonical_map, exact i+j, fapply bd_apprel,
+   exact push_to_sum_r x j, exact push_to_sum_l y i,
+    rw[<-H₁, <-H₂,<-Hx, <-Hy, <-canonical_map_quotient, same_fiber_as_push_to_r x j ,<-canonical_map_quotient, same_fiber_as_push_to_l y i],
+    simpa only},
+  {rcases f_ih_f₁ with ⟨t₁, H₁⟩, rcases f_ih_f₂ with ⟨t₂, H₂⟩,
+   rcases germ_rep t₁ with ⟨⟨i,x⟩,Hx⟩, rcases germ_rep t₂ with ⟨⟨j,y⟩,Hy⟩,
+   fapply exists.intro, fapply canonical_map, exact (i+j), fapply bd_imp,
+   exact push_to_sum_r x j, exact push_to_sum_l y i,
+    rw[<-H₁, <-H₂,<-Hx, <-Hy, <-canonical_map_quotient, same_fiber_as_push_to_r x j ,<-canonical_map_quotient, same_fiber_as_push_to_l y i],
+    simpa only},
+  {rcases f_ih with ⟨t₁, H₁⟩, rcases germ_rep t₁ with ⟨⟨i,x⟩,Hx⟩,
+   fapply exists.intro, fapply canonical_map, exact i, fapply bd_all,
+   exact x, rw[<-H₁, <-Hx], simpa only}},
+end
+
+@[simp]lemma bounded_formula'_comparison_bijective {L : Language} : function.bijective (@bounded_formula'_comparison L) :=
+by apply bounded_formula_comparison_bijective
+
+noncomputable def equiv_bounded_formula_comparison {L : Language} : equiv (colimit (@henkin_bounded_formula_chain' L)) (bounded_formula (L_infty L) 1) :=
+begin fapply equiv.of_bijective, exacts [bounded_formula'_comparison, bounded_formula'_comparison_bijective] end
+
+/- Not really a chain, since we haven't set up interpretations of theories yet -/
+def henkin_theory_chain {L : Language} (T : Theory L) : Π(n : ℕ), (Theory (obj (@henkin_language_chain L) n))
+| 0 := T
+| (n+1) := henkin_theory_step (henkin_theory_chain n)
+
+def is_consistent_henkin_theory_chain {L} {T : Theory L} (hT : is_consistent T) (n : ℕ) :
+  is_consistent (henkin_theory_chain T n) :=
+by induction n; [exact hT, exact is_consistent_henkin_theory_step n_ih]
+
+/- Now we have to push all these theories into Theory L_∞, so that they literally become a chain
+   of sets. -/
+
+/- Given T_n from henkin_theory_chain, ι T_n is the expansion of T_n to an L_infty theory -/
+def ι {L : Language} {T : Theory L} (m : ℕ) :  Theory (L_infty L) :=
+(Lhom.on_sentence (@henkin_language_canonical_map L m)) '' (@henkin_theory_chain L T m)
+
+@[simp]lemma in_iota_of_in_step {L} (i) {T} (f : sentence (@henkin_language_chain_objects L (i+1))): f ∈ (@henkin_theory_chain L T (i+1)) →  Lhom.on_bounded_formula (@henkin_language_canonical_map L (i + 1)) f ∈ @ι L T (i + 1) :=
+  by {intro H, split, swap, exact f, refine ⟨H,_⟩, refl}
+
+@[simp]lemma is_consistent_iota {L : Language} {T : Theory L} (hT : is_consistent T) (m : ℕ) : is_consistent (@ι _ T m) :=
+begin
+  unfold ι, intro a,
+  have := @is_consistent_henkin_theory_chain L T hT m,
+  suffices : (henkin_theory_chain T m) ⊢' bd_falsum, by contradiction,
+  apply nonempty.intro, apply reflect_prf,
+  exact henkin_language_canonical_map_inj m,
+  simp[on_formula, bounded_preformula.fst, Theory.fst, set.image_image, sprovable, on_sentence_fst] at *;
+  exact classical.choice a
+end
+
+@[simp]lemma not_succ (i : ℕ) : ¬ i = i + 1 :=
+by {have := nat.succ_ne_self i, tidy}
+
+lemma henkin_theory_chain_inclusion_step {L} {T : Theory L} {i : ℕ} {f ∈ henkin_theory_chain T i} :
+  (henkin_bounded_formula_chain 0 0).mor (nat.le_succ _) f ∈
+  henkin_theory_chain T (i + 1) :=
+begin
+dsimp[henkin_bounded_formula_chain, henkin_theory_chain],
+apply or.inl,
+unfold Theory_induced, fapply exists.intro, tidy,
+end
+
+lemma henkin_theory_chain_inclusion {L} {T : Theory L} {i j : ℕ} (h_leq : i ≤ j + 1) {f ∈ henkin_theory_chain T i} : (henkin_bounded_formula_chain 0 0).mor (by exact h_leq) f ∈ henkin_theory_chain T (j + 1) :=
+begin
+  dsimp[henkin_bounded_formula_chain],
+  by_cases i = j +1,
+    subst h, simp[id_bounded_formula 0 0 f], exact H,
+  induction j with j hj,
+  {
+    have : i = 0,
+    {suffices : i ≤ 0, by exact nat.eq_zero_of_le_zero this,
+      fapply nat.le_of_le_and_ne_succ, repeat{assumption}},
+    subst this,
+    apply or.inl, fapply exists.intro,
+    exact f, tidy
+  },
+  {
+    have hij : i ≤ nat.succ j,
+      by {fapply nat.le_of_le_and_ne_succ, repeat{assumption}},
+    -- have := hj hij,
+    by_cases i = j+1,
+       subst h, apply henkin_theory_chain_inclusion_step, assumption,
+    induction i with i hi,
+    {
+      unfold on_sentence henkin_language_chain_maps,
+      simp only [*, function.comp_app, on_bounded_formula, comp_on_bounded_formula, dif_neg, not_false_iff,
+        henkin_language_inclusion_chain_map],
+      apply or.inl, unfold Theory_induced,
+      fapply exists.intro,
+      {exact on_bounded_formula (henkin_language_chain_maps L (by assumption)) f},
+      {split, apply hj, assumption, dedup,
+        dsimp[on_sentence], unfold henkin_language_chain_maps, simp*},
+    },
+    {
+      unfold on_sentence henkin_language_chain_maps,
+      simp only [*, function.comp_app, on_bounded_formula, comp_on_bounded_formula, dif_neg, not_false_iff,
+        henkin_language_inclusion_chain_map],
+      apply or.inl, unfold Theory_induced,
+      fapply exists.intro,
+      {exact on_bounded_formula (henkin_language_chain_maps L (by assumption)) f},
+      { split, apply hj, assumption,
+        dedup,
+        dsimp[on_sentence], unfold henkin_language_chain_maps, simp*},
+    },
+  },
+end
+
+@[simp]lemma iota_inclusion_of_le {L} {T : Theory L} : Π{i : ℕ} {j : ℕ} (h : i ≤ j), (@ι _ T i) ⊆ (@ι _ T j)
+| i 0 h :=  by rw[(nat.eq_zero_of_le_zero h)]
+| i (j+1) h := by {by_cases i = j+1, rw[h],
+                   have := (cocone_of_bounded_formula_L_infty 0 0).h_compat,
+                   have this' := @this i (j+1) (by simp*),
+                   dsimp[cocone_of_bounded_formula_L_infty] at this',
+                   dsimp[ι, on_sentence], show Language, exact L,
+                   intros ψ hψ, have hψ_w := classical.psigma_of_exists hψ,
+                   cases hψ_w with x Hx,
+                   refine ⟨(@henkin_bounded_formula_chain L 0 0).mor (by assumption) x,_⟩,
+                   split, {simp[henkin_theory_chain_inclusion, Hx]},
+                   simp, change (function.comp (on_bounded_formula
+                   (henkin_language_canonical_map (j + 1)))
+                   ((henkin_bounded_formula_chain 0 0).mor _)) x = ψ,
+                   rw[<-this'], exact Hx.right
+                   }
+
+/- T_infty is the henkinization of T; we define it to be the union ⋃ (n : ℕ), ι(T n). -/
+@[reducible]def T_infty {L : Language} (T : Theory L) : Theory (L_infty L) := set.Union (@ι L T)
+
+@[reducible]def henkin_language {L} {T : Theory L} {hT : is_consistent T} : Language := L_infty L
+
+local infix ` →ᴸ `:10 := Lhom -- \^L
+
+/- I dislike this proof, but I don't know how apply canonical_map_language otherwise... -/
+def henkin_language_over {L} {T : Theory L} {hT : is_consistent T} : L →ᴸ (@henkin_language L T hT) :=
+by {change (henkin_language_chain.obj (0 : ℕ)) →ᴸ colimit_language henkin_language_chain, apply canonical_map_language}
+
+lemma henkin_language_over_injective {L} {T : Theory L} {hT : is_consistent T} : Lhom.is_injective (@henkin_language_over L T hT) :=
+begin
+  split, all_goals{intro n, unfold henkin_language_over canonical_map_language, simp,
+  rw[<-canonical_map], fapply canonical_map_inj_of_transition_maps_inj, intros i j H,
+  dsimp[diagram_functions, diagram_relations, henkin_language_chain],
+  simp only [henkin_language_chain_maps_inj, Lhom.is_injective.on_function, Lhom.is_injective.on_relation]}
+end
+
+def complete_henkin_Theory_over {L : Language} (T : Theory L) (hT : is_consistent T) : Type u := Σ' T' : Theory_over T hT, has_enough_constants T'.val ∧ is_complete T'.val
+
+@[reducible]def henkinization {L : Language} {T : Theory L} (hT : is_consistent T) : Theory (@henkin_language L T hT) := T_infty T
+
+/-- Given an f : bounded_formula L_infty, return a Henkin witness for f, along with all the
+    data and conditions needed to obtain this witness --/
+noncomputable def wit_infty {L} {T : Theory L} {hT : is_consistent T} (f : bounded_formula (@henkin_language L T hT) 1) : Σ c : (@henkin_language L T hT).constants, Σ (f' : Σ' (x : colimit (@henkin_bounded_formula_chain' L)), bounded_formula'_comparison x = f), Σ' (f'' : coproduct_of_directed_diagram (@henkin_bounded_formula_chain' L)), ⟦f''⟧ = f'.fst ∧ c = (henkin_language_canonical_map (f''.fst + 1)).on_function  (wit' f''.snd) :=
+begin
+  have f_lift1 := classical.psigma_of_exists ((bounded_formula'_comparison_bijective).right f),
+  have f_lift2 := germ_rep (f_lift1.fst),
+  refine ⟨(henkin_language_canonical_map (f_lift2.fst.fst + 1)).on_function (wit' (f_lift2.fst.snd)), f_lift1,(f_lift2.fst), f_lift2.snd,rfl⟩,
+end
+
+
+
+@[simp]lemma henkinization_is_henkin {L : Language} {T : Theory L} (hT : is_consistent T) : has_enough_constants (henkinization hT) :=
+begin
+  apply has_enough_constants.intro,
+  unfold henkinization T_infty, intro f, have big_sigma := wit_infty f, rcases big_sigma with ⟨c, Hc⟩, refine ⟨c,_⟩,
+  rcases Hc with ⟨⟨f', Hf'⟩,⟨i, f''⟩, H⟩,
+  fapply nonempty.intro, fapply axm,
+  simp only [*, fol.subst_formula, fol.bounded_preterm.fst, set.mem_Union, set.mem_image, fol.subst0_bounded_formula_fst, fol.bounded_preformula.fst],
+  refine ⟨_,⟨(i+1),_⟩,_⟩,
+  {fapply Lhom.on_bounded_formula, exact (@henkin_language_chain L).obj (i+1),
+   fapply henkin_language_canonical_map, fapply wit_property, fapply Lhom.on_bounded_formula,
+   exact (@henkin_language_chain L).obj i, exact henkin_language_inclusion,
+   exact f'', exact (wit' f'')},
+  {fapply in_iota_of_in_step, fapply or.inr, tidy},
+  {
+    let c_infty := (bd_const ((henkin_language_canonical_map (i + 1)).on_function (wit' f''))),
+    have this1 : bounded_preformula.fst (∃' f) ⟹
+      (bounded_preformula.fst f)[bounded_preterm.fst
+          (bd_const ((henkin_language_canonical_map (i + 1)).on_function (wit' f''))) //
+        0] = bounded_preformula.fst ((∃' f) ⟹ f[c_infty/0]),
+    {
+      rw fst_imp,
+      simp only [fol.subst0_bounded_term, true_and, eq_self_iff_true],
+
+      sorry
+    },
+    rw this1,
+    suffices : (Lhom.on_bounded_formula (henkin_language_canonical_map (i + 1))
+         (wit_property (Lhom.on_bounded_formula henkin_language_inclusion f'') (wit' f''))) = (∃' f ⟹ f[c_infty /0]), by rw[this],
+    unfold wit_property at *, dsimp[c_infty], rw[<-canonical_map_quotient] at H,
+    dsimp only [on_bounded_formula] at H,
+    rw[<-Hf',<-H.left],
+    unfold bounded_formula'_comparison bounded_formula_comparison id,
+    rw[(@universal_map_property ℕ' (henkin_bounded_formula_chain') (cocone_of_bounded_formula'_L_infty) i f'')],
+    dsimp only [cocone_of_bounded_formula'_L_infty],
+    have this0 : henkin_language_canonical_map i = henkin_language_canonical_map (i+1) ∘ henkin_language_inclusion,
+    -- { have h := cocone_of_L_infty.h_compat,
+    { have a := @cocone_language.h_compat _ _
+        (@cocone_of_L_infty L) i (i+1) (nat.le_succ _),
+      dsimp only [cocone_of_L_infty, cocone_of_colimit_language,
+        henkin_language_chain] at a,
+      unfold henkin_language_canonical_map,
+      simp only [*, henkin_language_inclusion_chain_map],
+      exact a,},
+    rw[this0,Lhom.comp_on_bounded_formula],
+    have this1 : (function.comp (Lhom.on_bounded_formula (henkin_language_canonical_map (i + 1)))
+           (Lhom.on_bounded_formula henkin_language_inclusion) f'') =
+           Lhom.on_bounded_formula (henkin_language_canonical_map (i+1))
+             (Lhom.on_bounded_formula henkin_language_inclusion f''),
+    by refl,
+    rw[this1],
+    have this2 : (Lhom.on_bounded_formula (henkin_language_canonical_map (i + 1))
+           (Lhom.on_bounded_formula henkin_language_inclusion f''))[bd_const
+          ((henkin_language_canonical_map (i + 1)).on_function (wit' f'')) /0] =
+          (Lhom.on_bounded_formula (henkin_language_canonical_map (i + 1))
+           ((Lhom.on_bounded_formula henkin_language_inclusion f'')[bd_const
+           (wit' f'') /0])),
+    { sorry,
+      -- simp only [henkin_language_canonical_map,
+      --   canonical_map_language, canonical_inclusion_coproduct,
+      --   subst0_bounded_formula],
+
+    },
+    rw[this2],
+    have this3 : ∃' Lhom.on_bounded_formula (henkin_language_canonical_map (i + 1))
+          (Lhom.on_bounded_formula henkin_language_inclusion f'')
+          = Lhom.on_bounded_formula (henkin_language_canonical_map (i+1)) (∃' (Lhom.on_bounded_formula henkin_language_inclusion f'')),
+    by refl,
+    rw[this3],
+  }
+end
+
+noncomputable def directed_union_finset_lift {α β : Type*} (ι : α → set β) (Γ' : finset (set.Union ι)) (x ∈ Γ') : Σ' a : α, (ι a) x :=
+begin
+cases x with x H', have := classical.psigma_of_exists H',
+rcases this with ⟨S,a⟩, simp[*,-a] at a, cases a with a1 a2,
+have := classical.psigma_of_exists a1, cases this with a Ha,
+rw[← Ha] at a2, exact ⟨a, a2⟩
+end
+
+/- For every n, T_n is a theory over T in Theory L_infty -/
+def henkin_Theory_over {L} (T : Theory L) (hT : is_consistent T) (n : ℕ) : Theory_over (@ι _ T 0) (@is_consistent_iota L T hT 0) :=
+begin
+  refine ⟨@ι _ T n, _⟩, split, apply iota_inclusion_of_le (nat.zero_le _),
+  apply is_consistent_iota hT
+end
+
+def henkin_theory_schain {L} (T : Theory L) (hT : is_consistent T): set (Theory_over (@ι _ T 0) (@is_consistent_iota L T hT 0))
+:= {T' | ∃ k : ℕ, (@ι _ T k) = T'.val}
+
+/- (T ∪ set.sUnion (subtype.val '' Ts)) actually is (henkinization hT) -/
+lemma iota_union_rw {L} (T : Theory L) (hT : is_consistent T) :
+  (@ι _ T 0) ∪ ⋃₀(subtype.val '' henkin_theory_schain T hT)
+  = henkinization hT :=
+begin
+  ext, split,
+  intro a,
+  cases a,
+    { obtain ⟨ a_w, hl, hr⟩ := a, cases hr,
+      simp only [set.mem_Union, on_sentence] at *,
+      use 0,
+      refine ⟨ a_w , hl , _ ⟩,
+      simp only [on_sentence],
+    },
+    {
+      obtain ⟨ s , H , hxs ⟩ := a,
+      simp only [henkinization, T_infty],
+      delta ι,
+      refine ⟨ s , _ , hxs ⟩,
+      simp only [on_sentence, set.mem_range, on_bounded_formula],
+      obtain ⟨ ⟨a , a1⟩ , b , hrw ⟩ :=  H,
+      rw ← hrw,
+      sorry,
+    },
+    {sorry,
+    -- right, cases a_h with H₁ H₂, use a_w, refine ⟨_,‹_›⟩,
+    --   { unfold henkin_theory_schain, rw[set.mem_range] at H₁,
+    --     cases H₁ with n Hn, rw[set.mem_image], refine ⟨_,_⟩,
+    --     use a_w, tidy, apply is_consistent_iota; from ‹_› }
+    }, recover
+end
+
+/- henkin_theory_chain satisfies the chain condition -/
+lemma chain_henkin_theory_chain {L} (T : Theory L) (hT : is_consistent T) : zorn.chain Theory_over_subset (henkin_theory_schain T hT) :=
+begin
+  tidy, rename H_1_w i, rename H_w j,
+  by_cases i ≤ j, apply or.inr, apply iota_inclusion_of_le, exact h,
+  apply or.inl, suffices : j ≤ i, by {apply iota_inclusion_of_le, exact this},
+  revert h, simp only [not_le], apply nat.le_of_lt
+end
+
+lemma is_consistent_henkinization {L : Language} {T : Theory L} (hT : is_consistent T) :
+is_consistent (henkinization hT) :=
+begin
+  have := @consis_limit _ _ _ (henkin_theory_schain T hT), rw[iota_union_rw] at this,
+  exact this (chain_henkin_theory_chain T hT)
+end
+
+
+-- @[simp]lemma is_consistent_henkinization {L : Language} {T : Theory L} (hT : is_consistent T) : is_consistent (henkinization hT) :=
+-- begin
+  -- intro P, have := proof_compactness P,
+  -- have : ∃ k : ℕ, @ι L T k ⊢' bd_falsum,
+  -- {sorry}, -- again, this depends on picking a representative of a germ-eq class
+  --          -- on the induced colimit of formulas
+  --          -- remark(Floris): we need a lemma that if a directed union of theories proves f, then an element of it proves f.
+  -- cases this with k P', unfold ι at P',
+  -- apply is_consistent_henkin_theory_chain hT k,
+  -- apply nonempty.map (Lhom.reflect_prf (henkin_language_canonical_map_inj k)),
+  -- simp only [on_formula, bounded_preformula.fst, Theory.fst, set.image_image, sprovable,
+  --   on_sentence_fst] at P' ⊢, exact P'
+-- end
+
+@[reducible]noncomputable def completion_of_henkinization_core {L} {T : Theory L} (hT : is_consistent T) : Σ' (T' : Theory_over (henkinization hT) _), is_complete (T'.val) := completion_of_consis _ (henkinization hT) (is_consistent_henkinization hT)
+
+/- the completed theory-/
+@[reducible]def completion_of_henkinization {L} {T : Theory L} (hT : is_consistent T) := (completion_of_henkinization_core (by assumption)).fst.val
+
+/- the completed theory contains the original theory -/
+@[simp]def completion_of_henkinization_contains {L} {T : Theory L} (hT : is_consistent T) := (completion_of_henkinization_core (by assumption)).fst.property.left
+
+/- the completed theory is consistent -/
+@[simp]def completion_of_henkinization_consistent {L} {T : Theory L} (hT : is_consistent T) := (completion_of_henkinization_core (by assumption)).fst.property.right
+
+/- the completed theory is complete -/
+@[reducible]def completion_of_henkinization_complete {L} {T : Theory L} (hT : is_consistent T) := (completion_of_henkinization_core (by assumption)).snd
+
+/- the completed theory is henkin -/
+@[simp]lemma completion_of_henkinization_is_henkin {L} {T : Theory L} (hT : is_consistent T) : has_enough_constants (completion_of_henkinization hT) :=
+begin
+fapply has_enough_constants.intro,
+  cases (@henkinization_is_henkin L T hT) with C H,
+  intro f, refine ⟨C f,_⟩, fapply weakening', exact (Theory.fst $ (henkinization hT)), fapply set.image_subset, simp, exact H f
+end
+
+/- The term model of the complete henkinization of T satisfies T -/
+@[simp]lemma reduct_of_complete_henkinization_models_T {L} {T : Theory L} (hT : is_consistent T) : Lhom.reduct (@henkin_language_canonical_map L 0) (term_model (completion_of_henkinization hT)) ⊨ T :=
+begin
+  fapply Lhom.reduct_all_ssatisfied,
+  {simp only [henkin_language_canonical_map_inj]}, intros f hf,
+  apply (term_model_ssatisfied (completion_of_henkinization_complete hT) (completion_of_henkinization_is_henkin hT)), fapply completion_of_henkinization_contains hT,
+  unfold henkinization T_infty, simp, refine ⟨0, _⟩, unfold ι, tidy
+end
+
+/- Given ψ ∈ T, the term model of the complete henkinization of T satisfies ψ -/
+@[simp]lemma reduct_of_complete_henkinization_satisfies {L} {T : Theory L} (hT : is_consistent T) (ψ : sentence L) (hψ : ψ ∈ T) : Lhom.reduct (@henkin_language_canonical_map L 0) (term_model (completion_of_henkinization hT)) ⊨ ψ :=
+  reduct_of_complete_henkinization_models_T _ hψ
